\documentclass[10pt, a4paper]{report}

\title{Cycling simulation}
\date{\today}
\author{Dan Demeter, Robert Kruszewski, Alex Paunoiu, C\'esar Prout\'e, Julian Sutherland}

\usepackage{tabularx, alltt, amsmath}

\begin{document}
\maketitle

% Initial equations

Runge-Kutta is a standard numerical method that allows one to estimate a function based on an initial value and its differential. Its a lot like the standard newton method ( basically $f(x + h) \approx f(x) + h*f'(x)$ ) but it uses several points inside a trapezium to trace the function significantly better.

However, you're going to say this is all very nice and it might well be useful for a first order differential equation, but we have a second order non-linear differential equation. Well one might notice that it is infact possible to adapt this method to tracing two (or more) interdependent functions (whos value depends on the value of the other) over the same variable (t) with two initial conditions. So if we can transform our second order differential equation into two first order ones, we can use Runge-Kutta to solve it numerically and then derive any necessary values from the result.

For the following equations we will use the next simbols: \\

\begin{tabularx}{\linewidth}{|c|X|}
\hline
P is power	&	\_pot is potential energy	\\
T is torque	&	\_air is air drag			\\
F is Force 	&  	\_bear is friction in the wheel bearings \\
			& 	\_roll is the rolling friction (with the road) \\
			& 	\_kin is kinetic energy \\
			&	\_ped is cyclist's 'input' (e.g. $P_{ped}$ = power inputed into the system) \\
\hline
\multicolumn{2}{|c|}
{
	$l_{c}$  is the length of the cycling crank and
	% maybe use a parbox here? http://tex.stackexchange.com/questions/485/how-to-break-a-line-in-a-table
	$r_{w}$  is the radius of the wheel
}

\end{tabularx}

\vspace*{1cm}

$\eta$ 		represents the frictional losses in the drive chain \\
$\omega$ 	represents angular velocity.\\
$\gamma$	is the step-up coefficient the bicycles gearing system.  \\

So by conservation of energy:

$$P_{pot} + P_{air} + P_{bear} + P_{roll} + P_{kin} = \eta * P_{ped}$$

As $Power = Torque * \omega$ , by dividing with $\omega$ we get

$$ T_{pot} + T_{air} + T_{bear} + T_{roll} + T_{kin} = \frac{ \eta * T_{ped} }{ \gamma }  = \frac{\eta * P_{ped}}{\omega * \gamma} $$

From the above notations have $T_{ped}$ = $F_{ped} * l_{c}$ (due to mechanical advantage) and $T = \frac{F * l_{c}}{r_{w}}$ for all the other forces (as there is a dual mechanical advantage between the crank and the wheel)

This gives us: $$ F_{pot} + F_{air} + F_{bear} + F_{roll} + F_{kin}
	= \frac{ \eta * l_{c} * T_{ped} }{ \gamma }
	= \frac{ \eta * l_{c} * P_{ped} }{ r_{w} * (\omega * \gamma)} $$

As we assume the race is on a perfectly flat surface, then $F_{pot} = 0$. We also assume that the bicycle is 'perfect', so $F_{bear} = 0$. \\\\
This simplifies to: $$F_{air} + F_{kin} = \frac{l_{c} * P_{ped} }{ \omega * \gamma } $$

where $$ F_{air} 	= \frac{1}{2} * c_{d} * \rho * A * ( x'(t) )^{2} $$
and	  $$ F_{kin} 	= ( m + ( \frac{l_w}{r_w^{2}} ) * x''(t) $$

Results from the Paper (...)\\

We are using the following estimates:

\begin{alltt}
mass of cyclist (m) 				= 63
frontal area of cyclist (A) 		= 0.75
length of crank (\(l_{c}\)) 		= 0.2
air density (\(\rho\)) 				= 1.225 (sea level, 15 degree Celsius)
drag coefficient of a cyclist (d) 	= 0.7
wheel inertia (\(I_w\)) = 0 (as perfect bicycle)
radius of wheel (\(r_w\)) = 0.35
step-up coefficient of gearing (\(\gamma\)) = 7.5
angular velocity of wheels (\(\omega\)) = \(2 * \pi * speed / {r_{w}} \)
\end{alltt}

Therefore the differential equation simplifies to:
$$ 0.3215625 * (x'(t))^{2} + 63 * x''(t)
	= \frac{\eta * l_{c} * P_{ped}} {2 * \pi * x'(t) * \gamma }
	= \frac {0.2 * P_{ped}} {15 * \pi} $$

Which gives approximation of:
$$ 75.7664 *(x'(t))^{3} + 14844.025288499999 * x'(t) * x''(t) = P_{ped}$$

which is a second order non-linear differential equation.\\\\
In order to apply the Runge-Kutta algorithm, we need to transform it into two linear differential equations. We will define 2 independent variables, $y_1$ and $y_2$ such that their differentials $y_1'$ and $y_2'$ must depend on the variables t, $y_1$ and $y_2$. Let
$$ y_1' = f( t, y_1, y_2 )$$ and $$y_2' = g( t, y_1, y_2 )$$

In order to get x'(t) we want to set one of the equations to contain it: $y_1 = x'(t)$ and because we want one of the equations to contain $x'(t) * x''(t) $ so set: $y_2' = x'( t ) * x''( t )$ .
This gives us $$ y_{2} = \frac{1}{2} * x'(t)^2 $$
By rearranging the differential equation to have only $ x'( t ) * x''( t )$ on the left hand side, we get
$$ x'( t ) * x''( t ) = \frac{P_{ped} - 75.7665 * x'( t ) ^ 3}{14844.025288499999}$$
$$ y_2' = \frac{P_{ped} - 75.7665 * x'( t ) ^ 3}{14844.025288499999}$$

Now we have only $y_2'$ in terms of only t, $y_1$ and $y_2$ so we can set $$ g( t, y_1, y_2 ) = \frac{P_{ped} - 75.7665 * x'( t ) ^ 3}{14844.025288499999}$$

Writing $y_1$ in terms of t, $y_1$ and $y_2$: $$y_2 = \frac{1}{2} * x'(t)^2$$ yelds $$y_2 = \frac{1}{2} * y_1^2$$
And by rearranging the left hand side we get:
$$y_1 = \sqrt{2 * y_2}$$
Now we differentiate with respect to $t$:
\begin{align*}
y_1' & = \frac{y_2'}{\sqrt{2 * y_2}}\\
& = \frac{P_{ped} - 75.7665 * x'( t ) ^ 3}{14844.025288499999 * \sqrt{2 * y_2}}
\end{align*}
This gives us the final form for function f:
$$ f(t, y_1, y_2) = \frac{P_{ped} - 75.7665 * x'( t ) ^ 3}{14844.025288499999 * \sqrt{2 * y_2}}$$

\end{document}
